nearly done optional.v

refinedVST/typing/optional.v
@@ -7,26 +7,29 @@ uses the same instances as Optionable.
   TODO: findout if there is a better way, maybe using Canonical Structures?
  *)
 
-Class Optionable `{!typeG OK_ty Σ} {cs : compspecs} (ty : type) (optty : type) (ot1 ot2 : Ctypes.type) := {
+Class Optionable `{!typeG OK_ty Σ} {cs : compspecs} (cty : Ctypes.type) (ty : type) (optty : type) (ot1 ot2 : Ctypes.type) := {
   opt_pre : val → val → iProp Σ;
   opt_bin_op (bty beq : bool) v1 v2 σ v :
-    (⊢ opt_pre v1 v2 -∗ (if bty then v1 ◁ᵥ ty else v1 ◁ᵥ optty) -∗ v2 ◁ᵥ optty -∗ juicy_mem.mem_auth σ -∗
+    (⊢ opt_pre v1 v2 -∗ (if bty then v1 ◁ᵥₐₗ|cty| ty else v1 ◁ᵥₐₗ|cty| optty) -∗ v2 ◁ᵥₐₗ|cty| optty -∗ juicy_mem.mem_auth σ -∗
       ⌜sem_binary_operation _ (if beq then Cop.Oeq else Cop.One) v1 ot1 v2 ot2 σ = Some v ↔ Vint (Int.repr (bool_to_Z (xorb bty beq))) = v⌝);
 }.
-Arguments opt_pre {_ _ _ _} _ {_ _ _ _} _ _.
+Arguments opt_pre {_ _ _ _ _} _ {_ _ _ _} _ _.
 
 Class OptionableAgree `{!typeG OK_ty Σ} {cs : compspecs} (ty1 ty2 : type) : Prop :=
   optionable_dist : True.
 
 Section optional.
-  Context `{!typeG OK_ty Σ} {cs : compspecs}.
+  Context `{!typeG OK_ty Σ} {cs : compspecs} (ge : genv).
+  Check opt_pre .
+  
+  Check Optionable.
 
   Global Program Instance optionable_ty_of_rty A (r : rtype A) `{!Inhabited A} optty ot1 ot2
-    `{!∀ x, Optionable (x @ r) optty ot1 ot2}: Optionable r optty ot1 ot2 := {|
-    opt_pre v1 v2 := (∀ x, opt_pre (x @ r) v1 v2)%I
+    `{!∀ x, Optionable cty (x @ r) optty ot1 ot2}: Optionable cty r optty ot1 ot2 := {|
+     opt_pre (v1 v2 : val) := (∀ x, opt_pre (x @ r) v1 v2)%I
   |}.
   Next Obligation.
-    iIntros(A r????? bty beq v1 v2 σ v) "Hpre Hv1 Hv2".
+    iIntros(A r?????? bty beq v1 v2 σ v) "Hpre Hv1 Hv2".
     unfold ty_of_rty; simpl_type.
     destruct bty. 1: iDestruct "Hv1" as (y) "Hv1".
     all: iApply (opt_bin_op with "Hpre [Hv1] Hv2") => /= //.
@@ -41,11 +44,13 @@ Section optional.
   Global Instance optionable_agree_id ty : OptionableAgree ty ty.
   Proof. done. Qed.
 
+  Check tptr.
+  
   (* Separate definition such that we can make it typeclasses opaque later. *)
-  Program Definition optional_type (ty : type) (optty : type) (b : Prop) : type := {|
+  Program Definition optional_type  (ty : type) (optty : type) (b : Prop) : type := {|
       ty_has_op_type ot mt := (ty.(ty_has_op_type) ot mt ∧ optty.(ty_has_op_type) ot mt)%type;
       ty_own β l := (<affine> ⌜b⌝ ∗ l◁ₗ{β}ty ∨ <affine> ⌜¬b⌝ ∗ l◁ₗ{β}optty)%I;
-      ty_own_val v := (<affine> ⌜b⌝ ∗ v ◁ᵥ ty ∨ <affine> ⌜¬b⌝ ∗ v ◁ᵥ optty)%I
+                                                                                 ty_own_val cty v := (<affine> ⌜b⌝ ∗ v ◁ᵥ|cty| ty ∨ <affine> ⌜¬b⌝ ∗ v ◁ᵥ|cty| optty)%I
   |}.
   Next Obligation.
     iIntros (??????).
@@ -55,7 +60,8 @@ Section optional.
     iIntros (ty?????[??]). by iDestruct 1 as "[[% Hv]|[% Hv]]";iDestruct (ty_aligned with "Hv") as %?.
   Qed.
   Next Obligation.
-    iIntros (ty?????[??]). by iDestruct 1 as "[[% Hv]|[% Hv]]";iDestruct (ty_size_eq with "Hv") as %?.
+    iIntros (ty?????[??]).
+    iDestruct 1 as "[[% Hv]|[% Hv]]";iDestruct (ty_size_eq with "Hv") as %?; eauto.
   Qed.
   Next Obligation.
     iIntros (ty optty ????[??]) "Hl".
@@ -66,7 +72,7 @@ Section optional.
     iDestruct "Hv" as "[[% Hv]|[% Hv]]"; iDestruct (ty_ref with "[] Hl Hv") as "H"; rewrite -?opt_alt_sz//;
        [iLeft | iRight]; by iFrame.
   Qed.
-(*   Next Obligation.
+(*  Next Obligation.
     iIntros (ty optty b v ot mt st [??]) "[[% Hv]|[% Hv]]".
     all: iDestruct (ty_memcast_compat with "Hv") as "Hv" => //.
     all: case_match => //. 1: iLeft. 2: iRight.
@@ -108,11 +114,16 @@ Section optional.
     iSplit => //. iApply (@simple_subsume_place with "HP Hl").
   Qed.
 
+  Check SimpleSubsumeVal.
+
   Global Instance simple_subsume_val_optional ty1 ty2 optty b1 b2
-       `{!Affine P} `{!SimpleSubsumeVal ty1 ty2 P}:
-    SimpleSubsumeVal (b1 @ optional ty1 optty) (b2 @ optional ty2 optty) (<affine> ⌜b1 ↔ b2⌝ ∗ P).
+       `{!Affine P} `{!SimpleSubsumeVal cty ty1 ty2 P}:
+    SimpleSubsumeVal cty (b1 @ optional ty1 optty) (b2 @ optional ty2 optty) (<affine> ⌜b1 ↔ b2⌝ ∗ P).
   Proof.
-    iIntros (v) "[Heq P] H". rewrite /ty_own_val /=. iDestruct "Heq" as %->.
+    iIntros (v) "[Heq P] H". rewrite /ty_own_val /=.
+    iDestruct "Heq" as "%Heq".
+    apply PropExtensionality.propositional_extensionality in Heq.
+    rewrite Heq.
     iDestruct "H" as "[[?H] | [??]]"; last (iRight; by iFrame).
     iLeft. iFrame. iApply (@simple_subsume_val with "P H").
   Qed.
@@ -134,15 +145,15 @@ Section optional.
   Definition subsume_optional_ty_ref_inst := [instance subsume_optional_ty_ref].
   Global Existing Instance subsume_optional_ty_ref_inst.
 
-  Lemma subsume_optional_val_optty_ref A b ty optty v T:
-    (∃ x, <affine> ⌜¬ b x⌝ ∗ T x) ⊢ subsume (v ◁ᵥ optty) (λ x : A, v ◁ᵥ (b x) @ optional (ty x) optty) T.
+  Lemma subsume_optional_val_optty_ref A b cty ty optty v T:
+    (∃ x, <affine> ⌜¬ b x⌝ ∗ T x) ⊢ subsume (v ◁ᵥ|cty| optty) (λ x : A, v ◁ᵥ|cty| (b x) @ optional (ty x) optty) T.
   Proof. iIntros "[% [Hb ?]] Hl". iExists _. iFrame. iRight. by iFrame. Qed.
   Definition subsume_optional_val_optty_ref_inst := [instance subsume_optional_val_optty_ref].
   Global Existing Instance subsume_optional_val_optty_ref_inst.
 
-  Lemma subsume_optional_val_ty_ref A b ty ty' optty v `{!∀ x, OptionableAgree (ty x) ty'} T:
-    (v ◁ᵥ ty' -∗ ∃ x, v ◁ᵥ ty x ∗ <affine> ⌜b x⌝ ∗ T x)
-    ⊢ subsume (v ◁ᵥ ty') (λ x : A, v ◁ᵥ (b x) @ optional (ty x) (optty x)) T.
+  Lemma subsume_optional_val_ty_ref A b cty ty ty' optty v `{!∀ x, OptionableAgree (ty x) ty'} T:
+    (v ◁ᵥ|cty| ty' -∗ ∃ x, v ◁ᵥ|cty| ty x ∗ <affine> ⌜b x⌝ ∗ T x)
+      ⊢ subsume (v ◁ᵥ|cty| ty') (λ x : A, v ◁ᵥ|cty| (b x) @ optional (ty x) (optty x)) T.
   Proof.
     iIntros "Hsub Hl". iDestruct ("Hsub" with "Hl") as (?) "[? [% ?]]".
     iExists _. iFrame. iLeft. by iFrame.
@@ -154,14 +165,18 @@ Section optional.
   | TraceOptionalEq (P : Prop)
   | TraceOptionalNe (P : Prop).
 
-  Lemma type_eq_optional_refined ge v1 v2 ty optty ot1 ot2 `{!Optionable ty optty ot1 ot2} `{!Affine (v2 ◁ᵥ optty)} b (T : _ → _ → assert)
+  Check opt_pre.
+  
+  Lemma type_eq_optional_refined v1 v2 (cty : Ctypes.type) (ty optty : type) (ot1 ot2 : Ctypes.type)
+    `{!Optionable cty ty optty ot1 ot2}
+    `{!Affine (v2 ◁ᵥₐₗ|cty| optty)} b (T : _ → _ → assert)
     (* We'll throw away any ownership associated with v2 (e.g. through an ownership type), so it needs to be affine.
        We could require T to be absorbing instead. *)  :
     ⎡opt_pre ty v1 v2⎤ ∧
     case_if b
-      (li_trace (TraceOptionalEq b) (⎡v1 ◁ᵥ ty⎤ -∗ T (i2v (bool_to_Z false) tint) (false @ boolean tint)))
-      (li_trace (TraceOptionalEq (¬ b)) (⎡v1 ◁ᵥ optty⎤ -∗ T (i2v (bool_to_Z true) tint) (true @ boolean tint)))
-    ⊢ typed_bin_op ge v1 ⎡v1 ◁ᵥ b @ (optional ty optty)⎤ v2 ⎡v2 ◁ᵥ optty⎤ Oeq ot1 ot2 T.
+      (li_trace (TraceOptionalEq b) (⎡v1 ◁ᵥₐₗ|cty| ty⎤ -∗ T (i2v (bool_to_Z false) tint) (false @ boolean tint)))
+      (li_trace (TraceOptionalEq (¬ b)) (⎡v1 ◁ᵥₐₗ|cty| optty⎤ -∗ T (i2v (bool_to_Z true) tint) (true @ boolean tint)))
+      ⊢ typed_bin_op ge v1 ⎡v1 ◁ᵥₐₗ|cty| b @ (optional ty optty)⎤ v2 ⎡v2 ◁ᵥₐₗ|cty| optty⎤ Oeq ot1 ot2 tint  T.
   Proof.
     iIntros "HT Hv1 Hv2" (Φ) "HΦ".
     iDestruct "Hv1" as "[[% Hv1]|[% Hv1]]".
@@ -173,9 +188,12 @@ Section optional.
         iDestruct (opt_bin_op true true with "Hpre Hv1 Hv2 Hctx") as %Hiff.
         iPureIntro; intros. simpl in Hiff. rewrite Hiff //.
       }
-      iDestruct "HT" as "[_ [HT _]]". iFrame.
-      iDestruct ("HT" with "[//] Hv1") as "HT".
-      iApply ("HΦ" with "[] HT"). by iExists _.
+      rewrite bi.and_elim_r.
+      iDestruct "HT" as "[HT _]". iFrame.
+      iSpecialize ("HΦ" $! (i2v (bool_to_Z false) _ ) (false @ boolean tint)).
+      iApply ("HΦ" with "[]").
+      { rewrite /ty_own_val_at /ty_own_val /=. iSplit; auto. by iExists _. }
+      iApply ("HT" with "[] Hv1"); try done.
     - iIntros "!>" (?) "Hctx !>".
       iExists (i2v (bool_to_Z true) tint).
       iSplit. {
@@ -186,14 +204,16 @@ Section optional.
       }
       iDestruct "HT" as "[_ [_ HT]]". iFrame.
       iDestruct ("HT" with "[//] Hv1") as "HT".
-      iApply ("HΦ" with "[] HT"). by iExists _.
+      iApply ("HΦ" with "[] HT").
+      rewrite /ty_own_val_at /ty_own_val /=. iSplit; auto. by iExists _.
   Qed.
   Definition type_eq_optional_refined_inst := [instance type_eq_optional_refined].
   Global Existing Instance type_eq_optional_refined_inst.
 
-  Lemma type_eq_optional_neq ge v1 v2 ty optty ot1 ot2 `{!Optionable ty optty ot1 ot2} `{!Affine (v2 ◁ᵥ optty)} T :
-    ⎡opt_pre ty v1 v2⎤ ∧ (∀ v, ⎡v1 ◁ᵥ ty⎤ -∗ T v (false @ boolean tint))
-    ⊢ typed_bin_op ge v1 ⎡v1 ◁ᵥ ty⎤ v2 ⎡v2 ◁ᵥ optty⎤ Oeq ot1 ot2 T.
+  Lemma type_eq_optional_neq v1 v2 (cty : Ctypes.type) ty optty ot1 ot2
+    `{!Optionable cty ty optty ot1 ot2} `{!Affine (v2 ◁ᵥₐₗ|cty| optty)} T :
+    ⎡opt_pre ty v1 v2⎤ ∧ (∀ v, ⎡v1 ◁ᵥₐₗ|cty| ty⎤ -∗ T v (false @ boolean tint))
+                           ⊢ typed_bin_op ge v1 ⎡v1 ◁ᵥₐₗ|cty| ty⎤ v2 ⎡v2 ◁ᵥₐₗ|cty| optty⎤ Oeq ot1 ot2 tint T.
   Proof.
     iIntros "HT Hv1 Hv2". iIntros (Φ) "HΦ".
     iIntros "!>" (?) "Hctx !>".
@@ -205,17 +225,19 @@ Section optional.
         iPureIntro; intros. simpl in Hiff. rewrite Hiff //.
     }
     iDestruct ("HT" with "Hv1") as "HT". iFrame.
-    iApply "HΦ" => //. iExists _. iSplit; iPureIntro; done.
+    iApply "HΦ" => //.
+    rewrite /ty_own_val_at /ty_own_val /=. iSplit; auto. by iExists _.
   Qed.
   Definition type_eq_optional_neq_inst := [instance type_eq_optional_neq].
   Global Existing Instance type_eq_optional_neq_inst.
 
-  Lemma type_neq_optional ge v1 v2 ty optty ot1 ot2 `{!Optionable ty optty ot1 ot2} `{!Affine (v2 ◁ᵥ optty)} b T :
+  Lemma type_neq_optional v1 v2 (cty : Ctypes.type) ty optty ot1 ot2
+    `{!Optionable cty ty optty ot1 ot2} `{!Affine (v2 ◁ᵥₐₗ|cty| optty)} b T :
     ⎡opt_pre ty v1 v2⎤ ∧
     case_if b
-      (li_trace (TraceOptionalNe b) (⎡v1 ◁ᵥ ty⎤ -∗ T (i2v (bool_to_Z true) tint) (true @ boolean tint)))
-      (li_trace (TraceOptionalNe (¬ b)) (⎡v1 ◁ᵥ optty⎤ -∗ T (i2v (bool_to_Z false) tint) (false @ boolean tint)))
-    ⊢ typed_bin_op ge v1 ⎡v1 ◁ᵥ b @ (optional ty optty)⎤ v2 ⎡v2 ◁ᵥ optty⎤ Cop.One ot1 ot2 T.
+      (li_trace (TraceOptionalNe b) (⎡v1 ◁ᵥₐₗ|cty| ty⎤ -∗ T (i2v (bool_to_Z true) tint) (true @ boolean tint)))
+      (li_trace (TraceOptionalNe (¬ b)) (⎡v1 ◁ᵥₐₗ|cty| optty⎤ -∗ T (i2v (bool_to_Z false) tint) (false @ boolean tint)))
+      ⊢ typed_bin_op ge v1 ⎡v1 ◁ᵥₐₗ|cty| b @ (optional ty optty)⎤ v2 ⎡v2 ◁ᵥₐₗ|cty| optty⎤ Cop.One ot1 ot2 tint T.
   Proof.
     unfold li_trace. iIntros "HT Hv1 Hv2" (Φ) "HΦ".
     iDestruct "Hv1" as "[[% Hv1]|[% Hv1]]".
@@ -229,7 +251,8 @@ Section optional.
       }
       iDestruct "HT" as "[_ [HT _]]". iFrame.
       iDestruct ("HT" with "[//] Hv1") as "HT".
-      iApply ("HΦ" with "[] HT"). by iExists _.
+      iApply ("HΦ" with "[] HT").
+      rewrite /ty_own_val_at /ty_own_val /=. iSplit; auto. by iExists _.
     - iIntros "!>" (?) "Hctx !>".
       iExists (i2v (bool_to_Z false) tint).
       iSplit. {
@@ -240,11 +263,13 @@ Section optional.
       }
       iDestruct "HT" as "[_ [_ HT]]". iFrame.
       iDestruct ("HT" with "[//] Hv1") as "HT".
-      iApply ("HΦ" with "[] HT"). by iExists _.
+      iApply ("HΦ" with "[] HT").
+      rewrite /ty_own_val_at /ty_own_val /=. iSplit; auto. by iExists _.
   Qed.
   Definition type_neq_optional_inst := [instance type_neq_optional].
   Global Existing Instance type_neq_optional_inst.
 
+  (*
   Global Program Instance optional_copyable b ty optty `{!Copyable ty} `{!Copyable optty} : Copyable (b @ optional ty optty).
   Next Obligation.
     iIntros (b ty optty ? ? E ly l ? [??]) "[[% Hl]|[% Hl]]".
@@ -253,6 +278,7 @@ Section optional.
     - by iLeft; iFrame.
     - by iRight; iFrame.
   Qed.
+  *)
 
 End optional.
 Global Typeclasses Opaque optional_type optional.
@@ -263,39 +289,44 @@ Notation "'optional' == ... : P" := (TraceOptionalEq P) (at level 100, only prin
 Notation "'optional' != ... : P" := (TraceOptionalNe P) (at level 100, only printing).
 
 Section optionalO.
-  Context `{!typeG OK_ty Σ} {cs : compspecs}.
+  Context `{!typeG OK_ty Σ} {cs : compspecs} (ge: genv).
     (* Separate definition such that we can make it typeclasses opaque later. *)
-  Program Definition optionalO_type {A : Type} (ty : A → type) (optty : type) (b : option A) : type := {|
+  Program Definition optionalO_type {A : Type} (cty : Ctypes.type) (ty : A → type) (optty : type) (b : option A) : type := {|
       ty_has_op_type ot mt := ((∀ x, (ty x).(ty_has_op_type) ot mt) ∧ optty.(ty_has_op_type) ot mt)%type;
       ty_own β l := (if b is Some x return _ then l◁ₗ{β}(ty x) else l◁ₗ{β}optty)%I;
-      ty_own_val v := (if b is Some x return _ then v ◁ᵥ (ty x) else v ◁ᵥ optty)%I
+      ty_own_val cty v := (if b is Some x return _ then v ◁ᵥ|cty| (ty x) else v ◁ᵥ|cty| optty)%I
   |}.
   Next Obligation.
-    iIntros (A ty? [x|]); apply ty_share.
+    iIntros (A ty ??????). destruct b; by apply ty_share.
   Qed.
   Next Obligation.
-    iIntros (A ty? [x|] ???[Hty ?]) "Hv";iDestruct (ty_aligned with "Hv") as %Ha => //.
+    iIntros (A ty ??????(?&?)) "Hv".
+    destruct b; iDestruct (ty_aligned with "Hv") as %Ha => //.
   Qed.
   Next Obligation.
-    iIntros (A ty? [x|] ???[??]) "Hv";iDestruct (ty_size_eq with "Hv") as %Ha => //.
+    iIntros (A ty ??????(?&?)) "Hv".
+    destruct b; iDestruct (ty_size_eq with "Hv") as %Ha => //.
   Qed.
   Next Obligation.
-    iIntros (A ty optty [] ?? l[??]) "Hl"; rewrite /with_refinement/ty_own/=; iDestruct (ty_deref with "Hl") as (?) "[? ?]"; eauto with iFrame.
+    iIntros (A ty optty?[]???[??]) "Hl"; rewrite /with_refinement/ty_own/=; iDestruct (ty_deref with "Hl") as (?) "[? ?]"; eauto with iFrame.
   Qed.
   Next Obligation.
-    iIntros (A ty optty [] ?? l v [??]?) "Hl Hv"; iApply (ty_ref with "[] Hl Hv") => //.
+    iIntros (A ty optty?[]????[??]?) "Hl Hv"; iApply (ty_ref with "[] Hl Hv") => //.
   Qed.
 (*   Next Obligation.
     iIntros (A ty optty [x|] v ot mt st [??]) "Hl".
     all: by iDestruct (ty_memcast_compat with "Hl") as "Hl".
   Qed. *)
 
-  Global Instance optionalO_type_le A : Proper (pointwise_relation A (⊑) ==> (⊑) ==> (eq) ==> (⊑)) optionalO_type.
+  Global Instance optionalO_type_le A cty:
+    Proper (pointwise_relation A (⊑) ==> (⊑) ==> (eq) ==> (⊑)) (optionalO_type cty).
   Proof. solve_type_proper. Qed.
-  Global Instance optionalO_type_proper A : Proper (pointwise_relation A (≡) ==> (≡) ==> (eq) ==> (≡)) optionalO_type.
+  Global Instance optionalO_type_proper A cty:
+    Proper (pointwise_relation A (≡) ==> (≡) ==> (eq) ==> (≡)) (optionalO_type cty).
   Proof. solve_type_proper. Qed.
 
-  Definition optionalO {A : Type} (ty : A → type) (optty : type) : rtype _ := RType (optionalO_type ty optty).
+  Definition optionalO {A : Type} cty (ty : A → type) (optty : type) : rtype _ :=
+    RType (optionalO_type cty ty optty).
 
 (*   Global Instance optionalO_loc_in_bounds A (ty : A → type) e ot β n `{!∀ x, LocInBounds (ty x) β n} `{!LocInBounds ot β n}:
     LocInBounds (e @ optionalO ty ot) β n.
@@ -305,47 +336,47 @@ Section optionalO.
   Qed. *)
 
   (* TODO: should be allow different opttys? *)
-  Global Instance simple_subsume_place_optionalO A (ty1 : A → _) ty2 optty b
+  Global Instance simple_subsume_place_optionalO A cty (ty1 : A → _) ty2 optty b
     `{!Affine P} `{!∀ x, SimpleSubsumePlace (ty1 x) (ty2 x) P}:
-    SimpleSubsumePlace (b @ optionalO ty1 optty) (b @ optionalO ty2 optty) P.
+    SimpleSubsumePlace (b @ optionalO cty ty1 optty) (b @ optionalO cty ty2 optty) P.
   Proof.
     iIntros (l β) "HP Hl". destruct b. 2: by iFrame.
     unfold optionalO; simpl_type. iApply (@simple_subsume_place with "HP Hl").
   Qed.
 
   (* TODO: Should we have more instances like this? E.g. for the goal? *)
-  Lemma simpl_hyp_optionalO_Some A (ty : A → type) optty l β x T:
-    (l ◁ₗ{β} ty x -∗ T) ⊢ simplify_hyp (l ◁ₗ{β} Some x @ optionalO ty optty) T.
+  Lemma simpl_hyp_optionalO_Some A cty (ty : A → type) optty l β x T:
+    (l ◁ₗ{β} ty x -∗ T) ⊢ simplify_hyp (l ◁ₗ{β} Some x @ optionalO cty ty optty) T.
   Proof. iIntros "HT Hl". by iApply "HT". Qed.
   Definition simpl_hyp_optionalO_Some_inst := [instance simpl_hyp_optionalO_Some with 0%N].
   Global Existing Instance simpl_hyp_optionalO_Some_inst.
-  Lemma simpl_hyp_optionalO_None A (ty : A → type) optty l β T:
-    (l ◁ₗ{β} optty -∗ T) ⊢ simplify_hyp (l ◁ₗ{β} None @ optionalO ty optty) T.
+  Lemma simpl_hyp_optionalO_None A cty (ty : A → type) optty l β T:
+    (l ◁ₗ{β} optty -∗ T) ⊢ simplify_hyp (l ◁ₗ{β} None @ optionalO cty ty optty) T.
   Proof. iIntros "HT Hl". by iApply "HT". Qed.
   Definition simpl_hyp_optionalO_None_inst := [instance simpl_hyp_optionalO_None with 0%N].
   Global Existing Instance simpl_hyp_optionalO_None_inst.
-  Lemma simpl_hyp_optionalO_Some_val A (ty : A → type) optty v x T:
-    (v ◁ᵥ ty x -∗ T) ⊢ simplify_hyp (v ◁ᵥ Some x @ optionalO ty optty) T.
+  Lemma simpl_hyp_optionalO_Some_val A cty (ty : A → type) optty v x T:
+    (v ◁ᵥ|cty| ty x -∗ T) ⊢ simplify_hyp (v ◁ᵥ|cty| Some x @ optionalO cty ty optty) T.
   Proof. iIntros "HT Hl". by iApply "HT". Qed.
   Definition simpl_hyp_optionalO_Some_val_inst := [instance simpl_hyp_optionalO_Some_val with 0%N].
   Global Existing Instance simpl_hyp_optionalO_Some_val_inst.
-  Lemma simpl_hyp_optionalO_None_val A (ty : A → type) optty v T:
-    (v ◁ᵥ optty -∗ T) ⊢ simplify_hyp (v ◁ᵥ None @ optionalO ty optty) T.
+  Lemma simpl_hyp_optionalO_None_val A cty (ty : A → type) optty v T:
+    (v ◁ᵥ|cty| optty -∗ T) ⊢ simplify_hyp (v ◁ᵥ|cty| None @ optionalO cty ty optty) T.
   Proof. iIntros "HT Hl". by iApply "HT". Qed.
   Definition simpl_hyp_optionalO_None_val_inst := [instance simpl_hyp_optionalO_None_val with 0%N].
   Global Existing Instance simpl_hyp_optionalO_None_val_inst.
 
-  Lemma subsume_optionalO_optty B A (ty : B → A → type) optty l β b T:
+  Lemma subsume_optionalO_optty B A cty (ty : B → A → type) optty l β b T:
     (∃ x, <affine> ⌜b x = None⌝ ∗ T x)
-    ⊢ subsume (l ◁ₗ{β} optty) (λ x : B, l ◁ₗ{β} (b x) @ optionalO (ty x) optty) T.
+    ⊢ subsume (l ◁ₗ{β} optty) (λ x : B, l ◁ₗ{β} (b x) @ optionalO cty (ty x) optty) T.
   Proof. iIntros "[% [%Heq ?]] Hl". iExists _. iFrame. by rewrite Heq. Qed.
   Definition subsume_optionalO_optty_inst := [instance subsume_optionalO_optty].
   Global Existing Instance subsume_optionalO_optty_inst.
 
-  Lemma subsume_optionalO_ty B A (ty : B → A → type) optty l β b ty'
+  Lemma subsume_optionalO_ty B A cty (ty : B → A → type) optty l β b ty'
     `{!∀ x y, OptionableAgree (ty y x) ty'} T:
     (l ◁ₗ{β} ty' -∗ ∃ y x, <affine> ⌜b y = Some x⌝ ∗ l ◁ₗ{β} ty y x ∗ T y)
-    ⊢ subsume (l ◁ₗ{β} ty') (λ y : B, l ◁ₗ{β} (b y) @ optionalO (ty y) (optty y)) T.
+    ⊢ subsume (l ◁ₗ{β} ty') (λ y : B, l ◁ₗ{β} (b y) @ optionalO cty (ty y) (optty y)) T.
   Proof.
     iIntros "Hsub Hl". iDestruct ("Hsub" with "Hl") as (?? Heq) "[??]".
     iExists _. iFrame. by rewrite Heq.
@@ -353,16 +384,16 @@ Section optionalO.
   Definition subsume_optionalO_ty_inst := [instance subsume_optionalO_ty].
   Global Existing Instance subsume_optionalO_ty_inst.
 
-  Lemma subsume_optionalO_optty_val B A (ty : B → A → type) optty v b T:
-    (∃ x, <affine> ⌜b x = None⌝ ∗ T x) ⊢ subsume (v ◁ᵥ optty) (λ x : B, v ◁ᵥ (b x) @ optionalO (ty x) optty) T.
+  Lemma subsume_optionalO_optty_val B A cty (ty : B → A → type) optty v b T:
+    (∃ x, <affine> ⌜b x = None⌝ ∗ T x) ⊢ subsume (v ◁ᵥ|cty| optty) (λ x : B, v ◁ᵥ|cty| (b x) @ optionalO cty (ty x) optty) T.
   Proof. iIntros "[% [%Heq ?]] Hl". iExists _. iFrame. by rewrite Heq. Qed.
   Definition subsume_optionalO_optty_val_inst := [instance subsume_optionalO_optty_val].
   Global Existing Instance subsume_optionalO_optty_val_inst.
 
-  Lemma subsume_optionalO_ty_val B A (ty : B → A → type) optty v b ty'
+  Lemma subsume_optionalO_ty_val B A cty (ty : B → A → type) optty v b ty'
     `{!∀ y x, OptionableAgree (ty y x) ty'} T:
-    (v ◁ᵥ ty' -∗ ∃ y x, <affine> ⌜b y = Some x⌝ ∗ v ◁ᵥ ty y x ∗ T y)
-    ⊢ subsume (v ◁ᵥ ty') (λ y : B, v ◁ᵥ (b y) @ optionalO (ty y) (optty y)) T.
+    (v ◁ᵥ|cty| ty' -∗ ∃ y x, <affine> ⌜b y = Some x⌝ ∗ v ◁ᵥ|cty| ty y x ∗ T y)
+      ⊢ subsume (v ◁ᵥ|cty| ty') (λ y : B, v ◁ᵥ|cty| (b y) @ optionalO cty (ty y) (optty y)) T.
   Proof.
     iIntros "Hsub Hl". iDestruct ("Hsub" with "Hl") as (?? Heq) "[??]".
     iExists _. iFrame. by rewrite Heq.
@@ -370,11 +401,13 @@ Section optionalO.
   Definition subsume_optionalO_ty_val_inst := [instance subsume_optionalO_ty_val].
   Global Existing Instance subsume_optionalO_ty_val_inst.
 
-  Lemma subsume_optional_optionalO_val B ty optty b v T:
+  Lemma subsume_optional_optionalO_val B cty ty optty b v T:
     (∃ x, T x) ⊢
-    subsume (v ◁ᵥ b @ optional ty optty) (λ x : B, v ◁ᵥ optionalO (λ _ : (), ty) optty) T.
+      subsume (v ◁ᵥ|cty| b @ optional ty optty) (λ x : B, v ◁ᵥ|cty| optionalO cty (λ _ : (), ty) optty) T.
   Proof.
-    unfold optional; simpl_type. iIntros "[% ?] [[% ?]|[% ?]]";
+    rewrite /optional; simpl_type.
+    rewrite /ty_own_val_at /ty_own_val /=.
+    iIntros "[%?] [(% & ?)|(% & ?)]";
       iExists _; iFrame; [iExists (Some ())|iExists None]; iFrame.
   Qed.
   Definition subsume_optional_optionalO_val_inst := [instance subsume_optional_optionalO_val].
@@ -383,13 +416,14 @@ Section optionalO.
   Inductive trace_optionalO :=
   | TraceOptionalO.
 
-  Lemma type_eq_optionalO ge A v1 v2 (ty : A → type) optty ot1 ot2 `{!∀ x, Optionable (ty x) optty ot1 ot2}
-    `{!Affine (v2 ◁ᵥ optty)} b `{!Inhabited A} T :
-    ⎡opt_pre (ty (default inhabitant b)) v1 v2⎤ ∧
+  Lemma type_eq_optionalO A (v1 v2 : val) (cty : Ctypes.type) (ty : A → type) optty (ot1 ot2 : Ctypes.type)
+    `{!∀ x, Optionable cty (ty x) optty ot1 ot2}
+    `{!Affine (v2 ◁ᵥₐₗ|cty| optty)} (b : option A) `{!Inhabited A} (T : _ → _ → assert):
+   ⎡opt_pre (ty (default inhabitant b)) v1 v2⎤ ∧ 
     case_destruct b (λ b _,
-      li_trace (TraceOptionalO, b) (∀ v, ⎡if b is Some x then v1 ◁ᵥ ty x else v1 ◁ᵥ optty⎤ -∗
+        li_trace (TraceOptionalO, b) (∀ v, ⎡if b is Some x then v1 ◁ᵥₐₗ|cty| ty x else v1 ◁ᵥₐₗ|cty| optty⎤ -∗
          T v ((if b is Some x then false else true) @ boolean tint)))
-    ⊢ typed_bin_op ge v1 ⎡v1 ◁ᵥ b @ optionalO ty optty⎤ v2 ⎡v2 ◁ᵥ optty⎤ Oeq ot1 ot2 T.
+      ⊢ typed_bin_op ge v1 ⎡v1 ◁ᵥₐₗ|cty| b @ optionalO cty ty optty⎤ v2 ⎡v2 ◁ᵥₐₗ|cty| optty⎤ Oeq ot1 ot2 cty T.
   Proof.
     unfold li_trace. iIntros "HT Hv1 Hv2". iIntros (Φ) "HΦ".
     destruct b.
